LC2996Assignment.lean
@@ -1,5 +1,5 @@
 import LC2996Assignment.Grader
 import LC2996Assignment.Student
 
-#eval LC2996.Student.smallestMissingNatGtSequentialPrefixSum [1,2,3,2,5]
-#eval LC2996.Student.smallestMissingNatGtSequentialPrefixSum [3,4,5,1,12,14,13]
+-- #eval LC2996.Student.smallestMissingNatGeSequentialPrefixSum [1,2,3,2,5]
+-- #eval LC2996.Student.smallestMissingNatGeSequentialPrefixSum [3,4,5,1,12,14,13]
